\documentclass{article}
\usepackage{epsfig}
\usepackage{/home/pengfei/OpenFOAM/OpenFOAM-v1912/doc/Doxygen/Macros/tensorOperator}
\pagestyle{empty}
\begin{document}
\[ U = \frac{U^*}{\kappa} ln\left(\frac{z - z_g + z_0}{z_0}\right) \]
\pagebreak

\[ k = \frac{(U^*)^2}{\sqrt{C_{\mu}}} \]
\pagebreak

\[ \epsilon = \frac{(U^*)^3}{\kappa(z - z_g + z_0)} \]
\pagebreak

$ U^* $
\pagebreak

$ \kappa $
\pagebreak

$ C_{\mu} $
\pagebreak

$ z $
\pagebreak

$ z_0 $
\pagebreak

$ z_g $
\pagebreak

\[ U^* = \kappa\frac{U_{ref}}{ln\left(\frac{Z_{ref} + z_0}{z_0}\right)} \]
\pagebreak

$ U_{ref} $
\pagebreak

$Z_{ref}$
\pagebreak

$ Z_{ref} $
\pagebreak

$\epsilon$
\pagebreak

$k$
\pagebreak

\[ U = \frac{U_f}{K} ln \left(\frac{z + z_0}{z_0}\right) \]
\pagebreak

$ U_f $
\pagebreak

$ K $
\pagebreak

\[ S = -\rho C_d \Sigma |U|^{(C_1 - 1)} U \]
\pagebreak

$ \Sigma $
\pagebreak

$ C_d $
\pagebreak

$ C_1 $
\pagebreak

\[ p = pa - \vec{g} & \vec{r} \]
\pagebreak

$ p $
\pagebreak

$ pa $
\pagebreak

$ g $
\pagebreak

\[ S = - (\mu d + \frac{\rho |U|}{2} f) U \]
\pagebreak

$ d $
\pagebreak

$ f $
\pagebreak

\[ S = - \rho_ref (\alpha + \beta |U|) U \]
\pagebreak

\[ S = - \rho C_0 |U|^{(C_1 - 1)} U \]
\pagebreak

$ C_0 $
\pagebreak

\[ S = - \alpha \rho D(T) U \]
\pagebreak

$ \alpha $
\pagebreak

$ D(T) $
\pagebreak

\[ U_p = cos(\theta) U_{Inf} + sin(\theta) (n \times U_{Inf}) - U_{p,srf} \]
\pagebreak

$ U_p $
\pagebreak

$ U_{Inf} $
\pagebreak

$ \theta $
\pagebreak

$ n $
\pagebreak

$ U_{p,srf} $
\pagebreak

\[ U_p = U_{in} \]
\pagebreak

\[ U_p = U_{in} - U_{p,srf} \]
\pagebreak

$ U_{in} $
\pagebreak

\[ U_p = - U_{p,srf} \]
\pagebreak

$ U_p = patch velocity [m/s]$
\pagebreak

$ U_{p,srf} = SRF velocity$
\pagebreak

\[ x_p = x_c + \frac{\nabla(x)}{\Delta} \]
\pagebreak

$ x_p $
\pagebreak

$ x_c $
\pagebreak

$ \nabla(x)$
\pagebreak

$ \Delta $
\pagebreak

\[ x_p = w x_p + (1-w) \left(x_c + \frac{\nabla_\perp x}{\Delta}\right) \]
\pagebreak

$ \Delta$
\pagebreak

$ w $
\pagebreak

\[ x = x_{old} + sign(F_{net})\frac{dt}{DT} \]
\pagebreak

$ x $
\pagebreak

$ x_{old} $
\pagebreak

$ dt $
\pagebreak

$ DT $
\pagebreak

$ F_{net} $
\pagebreak

\[ x = x_{old} + s \times \frac{dt}{DT} \]
\pagebreak

$ s $
\pagebreak

\[ \rho = \rho_{l,sat} + \psi_l*(p - p_{sat}) \]
\pagebreak

$ \rho $
\pagebreak

$ \rho_{l,sat} $
\pagebreak

$ \psi_l $
\pagebreak

$ p_{sat} $
\pagebreak

\[ U_p = U_c - n (n \cdot U_c) + \frac{n \phi_p}{|S_f|} \]
\pagebreak

$ U_c $
\pagebreak

$ \phi_p $
\pagebreak

$ S_f $
\pagebreak

\[ p_{hyd} = p_{ref} + \rho g (x - x_{ref}) \]
\pagebreak

$ p_{hyd} $
\pagebreak

$ p_{ref} $
\pagebreak

$ x_{ref} $
\pagebreak

$p_{hyd}$
\pagebreak

\[ p_rgh = p - \rho g (h - hRef) \]
\pagebreak

$ p_rgh $
\pagebreak

$ h $
\pagebreak

$ hRef $
\pagebreak

\[ p_rgh = ph_rgh - 0.5 \rho |U|^2 \]
\pagebreak

$ \rho g (h - h_{ref}) $
\pagebreak

$ ph_rgh $
\pagebreak

\[ p_rgh = p - \rho g.(h - hRef) \]
\pagebreak

\[ p = p0 - 0.5 \rho |U|^2 \]
\pagebreak

$ p0 $
\pagebreak

\[ p_p = p_0 - 0.5 |U|^2 \]
\pagebreak

$ p_p $
\pagebreak

$ p_0 $
\pagebreak

$ U $
\pagebreak

\[ p_p = p_0 - 0.5 \rho |U|^2 \]
\pagebreak

$\gamma = 1$
\pagebreak

\[ p_p = \frac{p_0}{1 + 0.5 \psi |U|^2} \]
\pagebreak

$ G $
\pagebreak

$\frac{\gamma}{1-\gamma}$
\pagebreak

$\gamma > 1$
\pagebreak

\[ p_p = \frac{p_0}{(1 + 0.5 \psi G |U|^2)^{\frac{1}{G}}} \]
\pagebreak

$ \gamma $
\pagebreak

$ \psi $
\pagebreak

\[ x_p = (1 - \alpha) x_p^{n - 1} + \alpha (x_{ref} + c s R |x_{ref}|) \]
\pagebreak

$ by heuristically adding a fraction of the new random component$
\pagebreak

$ to the previous time patch field$
\pagebreak

$ c $
\pagebreak

$ to compensate energy level losses due to the alpha scalar$
\pagebreak

$ R $
\pagebreak

\[ k_p = 1.5 (I |U|)^2 \]
\pagebreak

$ k_p $
\pagebreak

$ I $
\pagebreak

\[ p = -\rho*g*\zeta \]
\pagebreak

$ \zeta $
\pagebreak

\[ w_p = \frac{\phi_p}{|Sf|} + \sqrt{\frac{\gamma}{\psi_p}} \]
\pagebreak

$ w_p $
\pagebreak

$ \psi_p $
\pagebreak

$ Sf $
\pagebreak

\[ weight = 1 - max(min((Co - Co1)/(Co2 - Co1), 1), 0) \]
\pagebreak

$ Co1 $
\pagebreak

$ Co2 $
\pagebreak

\[ weight = f scheme1 + (1 - f) scheme2 \]
\pagebreak

\[ p' = \frac{1}{4 \pi c_0}\frac{\vec d}{|\vec d|^2}\frac{d(F)}{d(t)} \]
\pagebreak

$ p' $
\pagebreak

$ c_0 $
\pagebreak

$ \vec d $
\pagebreak

$ F $
\pagebreak

\[ \overline{x} = \frac{1}{N}\displaystyle\sum\limits_{i=0}^N x_i \]
\pagebreak

\[ \overline{x'}^2 = \frac{1}{N}\displaystyle\sum\limits_{i=0}^N (x_i - \overline{x})^2 \]
\pagebreak

$N$
\pagebreak

\[ UI(\phi) = 1 - \frac{1}{2 \overline{\phi} A} \int{\left| W \phi \cdot \hat{n} - \bar{W} \bar{\phi}\right| d\vec{A}} \,,\; \bar{\phi} = \frac{\int{W \phi \cdot d\vec{A}}}{\int{W \cdot d\vec{A}}} \]
\pagebreak

$ \phi = \vec{U} $
\pagebreak

$ \rho \vec{U} $
\pagebreak

$ \vec{U} $
\pagebreak

$ \phi = conc $
\pagebreak

\[ h = \frac{q}{T_{ref} - T_w} \]
\pagebreak

\[ h = \frac{q}{T_c - T_w} \]
\pagebreak

\[ C_f = \frac{\tau_w}{0.5 \rho_\infty |U|^2} \]
\pagebreak

\[ h = 0.5 \rho_\infty C_{p,\infty} |U_{\infty}| C_f \]
\pagebreak

\[ p_s = p_{ref} + \rho p_k \]
\pagebreak

\[ p_0 = p_{ref} + p + 0.5 \rho |U|^2 \]
\pagebreak

\[ p_i = p*(1 + ((gamma-1)*M^2)/2)^(gamma/(gamma - 1)) \]
\pagebreak

\[ Cp = \frac{p_s - p_{\inf}}{0.5 \rho_{\inf} |U_{\inf}|^2} \]
\pagebreak

\[ Cp_0 = \frac{p_0 - p_{\inf}}{0.5 \rho_{\inf} |U_{\inf}|^2} \]
\pagebreak

$ \rho_{\inf} $
\pagebreak

$ p_{\inf} $
\pagebreak

$ U_{\inf} $
\pagebreak

$ p_k $
\pagebreak

$ p_s $
\pagebreak

$ p_i $
\pagebreak

$ Cp $
\pagebreak

$ Cp_0 $
\pagebreak

$ \rho (\vec{g} \dot \vec{h})$
\pagebreak

$ P_A $
\pagebreak

$ k $
\pagebreak

$ \epsilon $
\pagebreak

\[ P_A = alpha_\epsilon \rho \epsilon M_t^5 \]
\pagebreak

$ alpha_\epsilon $
\pagebreak

\[ M_t = \frac{\sqrt{2 k}}{a_0} \]
\pagebreak

$ a_0 $
\pagebreak

\[ L_P = 10 \log \frac{P_A}{P_ref} \]
\pagebreak

$ P_ref $
\pagebreak

\[ Q = 0.5(sqr(tr(\nabla U)) - tr(((\nabla U) \cdot (\nabla U)))) \]
\pagebreak

\[ ref_c = s(f_{c}(t) - f_p + f_{off}) \]
\pagebreak

$ ref_c $
\pagebreak

$ f_{c}(t) $
\pagebreak

$ f_p $
\pagebreak

$ f_{off} $
\pagebreak

\[ fNon = min ( max ( 0.0, (nonOrthogonality - maxNonOrthogonality) /(minNonOrthogonality - maxNonOrthogonality) ), 1.0 ) \]
\pagebreak

\[ fMagGradCc = min ( max ( 0.0, (magGradCC - maxGradCc) / (minGradCc - maxGradCc) ), 1.0 ) \]
\pagebreak

\[ factor = P*residual + I*residualIntegral + D*residualDifferential \]
\pagebreak

\[ fRes = (factor - meanRes)/(maxRes*meanRes); \]
\pagebreak

\[ ffaceWeight = min ( max ( 0.0, (minFaceWeight - faceWeights) / (minFaceWeight - maxFaceWeight) ), 1.0 ) \]
\pagebreak

\[ fskewness = min ( max ( 0.0, (skewness - maxSkewness) / (minSkewness - maxSkewness) ), 1.0 ) \]
\pagebreak

\[ fCoWeight = min(max((Co - Co1)/(Co2 - Co1), 0), 1) \]
\pagebreak

\[ f = max(fNon, fMagGradCc, fRes, ffaceWeight, fskewness, fCoWeight) \]
\pagebreak

\[ Stress = R \dot n \]
\pagebreak

\[ Nu = 2.0 + \left(0.4 Re^{0.5} + 0.06 Re^{2/3}\right)*Pr^{0.4} \]
\pagebreak

$ autoWrite $
\pagebreak

$ noWrite $
\pagebreak

$ anyWrite $
\pagebreak

\[ T = 2 \rho A U_{o}^2 a (1-a) \]
\pagebreak

\[ U_1 = (1 - a)U_{o} \]
\pagebreak

$ A $
\pagebreak

$ U_o $
\pagebreak

$ a $
\pagebreak

$ U_1 $
\pagebreak

\[ Q_t = e(\phi, \dot{m}_2) (T_2 - T_1) \phi c_p \]
\pagebreak

$ Q_t $
\pagebreak

$ e(\phi,\dot{m}_2) $
\pagebreak

$ \phi $
\pagebreak

$ \dot{m}_2 $
\pagebreak

$ T_1 $
\pagebreak

$ T_2 $
\pagebreak

$ c_p $
\pagebreak

\[ Q_c = \frac{V_c |U_c| (T_c - T_{ref})}{\sum(V_c |U_c| (T_c - T_{ref}))} \]
\pagebreak

$ Q_c $
\pagebreak

$ V_c $
\pagebreak

$ T_c $
\pagebreak

$ T_{ref} $
\pagebreak

\[ \grad \left( \sigma \grad V \right) \]
\pagebreak

$ V $
\pagebreak

$\sigma$
\pagebreak

\[ \frac{d(P)}{d(V)} = J \cdot E \]
\pagebreak

$ J $
\pagebreak

$ E $
\pagebreak

\[ J = \sigma E \]
\pagebreak

\[ E = \grad V \]
\pagebreak

\[ \frac{d(P)}{d(V)} = J \cdot E = (sigma E) \cdot E = (sigma \grad V) \cdot \grad V \]
\pagebreak

\[ thrust(r) = T (C_0 + C_1 r^2 + C_2 r^4) \]
\pagebreak

\[ S(x) = S_u + S_p x \]
\pagebreak

$ S(x) $
\pagebreak

$ S_u $
\pagebreak

$ S_p $
\pagebreak

\[ -htc*Tmapped + Sp(htc, T) \]
\pagebreak

\[ htc = C_{min} \frac{NTU}{V_{core}} \]
\pagebreak

$ C_{min} $
\pagebreak

\[ C_{min} = min \left(Cp_1 \dot{m}_1, Cp_2 \dot{m}_2 \right) \]
\pagebreak

\[ cumulative model = (1.0 - exp( -(( x - d0)/d)^n ) / (1.0 - exp( -((d1 - d0)/d)^n ) \]
\pagebreak

\[ \Delta \phi = (A - B \phi^n) \frac{1}{B} (1 - e^{- B \Delta t}) \]
\pagebreak

\[ \Delta \phi = (A - B \phi^n) \frac{\Delta t}{1 + B \Delta t} \]
\pagebreak

\[ \frac{d \phi}{d t} = A - B \phi \]
\pagebreak

$\Delta t_e$
\pagebreak

\[ \Delta t_e = f(\Delta t, B) \]
\pagebreak

\[ \Delta \phi = (A - B \phi^n) \Delta t_e \]
\pagebreak

$A$
\pagebreak

$B$
\pagebreak

$\sum \alpha_i$
\pagebreak

$\sum \beta_i$
\pagebreak

\[ \frac{d \phi_i}{d t} = \alpha_i - \beta_i \phi \]
\pagebreak

\[ \Delta \phi_i = \alpha_i \Delta t - \beta_i \int_0^{\Delta t} \phi d t \]
\pagebreak

\[ \Delta \phi_i = (\alpha_i - \beta_i \phi^n) \Delta t - (A - B \phi^n) \int_0^{\Delta t} t_e dt \]
\pagebreak

$\int_0^{\Delta t} t_e dt$
\pagebreak

$e$
\pagebreak

\[ \frac{P_s \alpha^\beta}{ \mathrm{max} \left( \alpha_{pack} - \alpha , \epsilon ( 1 - \alpha ) \right) } \]
\pagebreak

$\alpha$
\pagebreak

\[ \left( \alpha \rho + \alpha^2 \rho (1 + e) \frac{3}{5} \left( 1 - \left( \frac{\alpha}{\alpha_{pack}} \right)^\frac{1}{3} \right) \right) \frac{1}{3} \sigma^2 \]
\pagebreak

$\rho$
\pagebreak

\[ V_d = V sqrt(epsilon)(B1 T + B2 T^2) \]
\pagebreak

\[ y_{n+1} = y_n + \delta_x f \]
\pagebreak

\[ err_{n+1} = y_{n+1} - y_n \]
\pagebreak

\[ y_{n+1} = y_n + \delta_x\left[I - \delta_x\frac{\partial f}{\partial y}\right]^{-1} \cdot \left[f(y_n) + \delta_x\frac{\partial f}{\partial x}\right] \]
\pagebreak

$ ax + by + cz + d = 0 $
\pagebreak

\[ a sin(2 \pi f (t - t_0)) s + l \]
\pagebreak

$ symbol $
\pagebreak

$ l $
\pagebreak

$ t_0 $
\pagebreak

$ t $
\pagebreak

\[ a square(f (t - t_0)) s + l \]
\pagebreak

$ square(t) $
\pagebreak

$ [-1, 1] $
\pagebreak

$ r $
\pagebreak

$k = c_{i,liq}/c_{i,gas}$
\pagebreak

\[ \log p = A + \frac{B}{C + T} \]
\pagebreak

$C$
\pagebreak

\[ \log (p) = A + \frac{B}{C + T} + D \log (T) + E T^F \]
\pagebreak

$D$
\pagebreak

$E$
\pagebreak

$F$
\pagebreak

$T_sat$
\pagebreak

\[ T_sat = \sum_i C_i p^i \]
\pagebreak

$p$
\pagebreak

\[ 0.5 d_j^{*^{5/3}} \mathrm{exp}\left(-\frac{\sqrt{2}}{d_j^{*^{3}}}\right) \frac{6}{\pi^{3/2}d_i^{*^{3}}} \mathrm{exp} \left( - \frac{9}{4}\left[\mathrm{ln}\left(2^{2/5} d_i^{*}\right)\right]^{2} \right) \left( 1 + \mathrm{erf} \left[ \frac{3}{2}\mathrm{ln} \left(2^{1/15} d_j^{*}\right) \right] \right)^{-1} \frac{1}{L^{3}T} \]
\pagebreak

\[ T = \left(\frac{\sigma}{\rho_c}\right)^{2/5} \frac{1}{\epsilon_c^{3/5}} \]
\pagebreak

\[ d^{*} = \frac{d}{L} \]
\pagebreak

\[ L = \left(\frac{\sigma}{\rho_c}\right)^{3/5} \frac{1}{\epsilon_c^{2/5}} \]
\pagebreak

$ \rho_c $
\pagebreak

$ \sigma $
\pagebreak

$ \epsilon_c $
\pagebreak

$ d_i $
\pagebreak

$ d_j $
\pagebreak

\[ C_4 \alpha_c \left(\frac{\epsilon_c}{d_j^2}\right)^{1/3} \int\limits_{\xi_{min}}^{1} \frac{\left(1 + \xi\right)^{2}}{\xi^{11/3}} \mathrm{exp} \left( - \frac{12c_f\sigma}{\beta\rho_c\epsilon_c^{2/3}d_j^{5/3}\xi^{11/3}} \right) \mathrm{d} \xi \]
\pagebreak

\[ c_f = \left(\frac{v_i}{v_j}\right)^{2/3} + \left(1 - \frac{v_i}{v_j}\right)^{2/3} - 1 \]
\pagebreak

\[ \xi_{min} = \frac{\lambda_{min}}{d_j}\,, \]
\pagebreak

\[ \lambda_{min} = C_5 \eta\,. \]
\pagebreak

\[ \frac{3}{11 b^{8/11}} \left( \left[\Gamma(8/11, b) - \Gamma(8/11, t_{m})\right] + 2b^{3/11} \left[\Gamma(5/11, b) - \Gamma(5/11, t_{m})\right] + b^{6/11} \left[\Gamma(2/11, b) - \Gamma(2/11, t_{m})\right] \right) \]
\pagebreak

\[ b = \frac{12c_f\sigma}{\beta\rho_c\epsilon_c^{2/3}d_j^{5/3}} \]
\pagebreak

\[ t_{min} = b \xi_{min}^{-11/3}\,. \]
\pagebreak

\[ \Gamma(a,z) = Q(a,z) \Gamma(a) \]
\pagebreak

$ \alpha_c $
\pagebreak

$ v_i $
\pagebreak

$ v_j $
\pagebreak

$ \xi $
\pagebreak

$ \xi_{min} $
\pagebreak

$ c_f $
\pagebreak

$ \eta $
\pagebreak

$ \Gamma(a,z) $
\pagebreak

$ Q(a,z) $
\pagebreak

$ \Gamma(a) $
\pagebreak

\[ C_1 \epsilon_c^{1/3} \mathrm{erfc} \left( \sqrt { C_2 \frac{\sigma}{\rho_c \epsilon_c^{2/3} (6v_i/\pi)^{5/9}} + C_3 \frac{\mu_c}{\sqrt{\rho_c \rho_d} \epsilon_c^{1/3} (6v_i/\pi)^{4/9}} } \right) \]
\pagebreak

$ \mu_c $
\pagebreak

$ \rho_d $
\pagebreak

\[ C_1 (v_i^{2/3} + v_j^{2/3}) (v_i^{2/9} + v_j^{2/9})^{1/2} \frac{\epsilon_c^{1/3}}{1 + \alpha_d} \text{exp} \left[ - C_2 \frac{\mu_c \rho_c}{\sigma^2} \frac{\epsilon_c}{(1 + \alpha_d)^{3}} \left( \frac{v_i^{1/3} v_j^{1/3}}{v_i^{1/3} + v_j^{1/3}} \right)^{4} \right] \]
\pagebreak

$ \alpha_d $
\pagebreak

\[ \frac{\pi}{4} (d_i + d_j)^2 \mathrm{min}(u^{\prime}, u_{\mathrm{crit}}) \mathrm{exp} \left[ - \left(\frac{\alpha_{\mathrm{max}}^{1/3}}{\alpha^{1/3}} - 1\right)^2 \right]\,, \]
\pagebreak

\[ u^{\prime} = \mathrm{max} \left( \sqrt{2} \epsilon_c^{1/3} \sqrt{d_i^{2/3} + d_j^{2/3}}, |\vec{u}_i - \vec{u}_j| \right) \]
\pagebreak

$ \alpha_{max} $
\pagebreak

$ u_{crit} $
\pagebreak

$ \vec{u}_i $
\pagebreak

$ \vec{u}_j $
\pagebreak

\[ &\frac{\pi}{4} (d_i + d_j)^2 u_{ij} \mathrm{exp} \left[ - C_1 \frac {[0.75(1 + \xi_{ij}^2)(1 + \xi_{ij}^3)]^{1/2}} {(\rho_d/\rho_c + C_{vm})^{1/2} (1 + \xi_{ij})^3} \left(\frac{\rho_c d_i u_{ij}^2}{\sigma}\right)^{1/2} \right]\,, \]
\pagebreak

\[ u_{ij} = \sqrt{\beta} (\epsilon_c d_i)^{1/3} \sqrt{1 + \xi_{ij}^{-2/3}} \]
\pagebreak

\[ \xi_{ij} = d_i/d_j \]
\pagebreak

$ u_{ij} $
\pagebreak

$ \xi_{ij} $
\pagebreak

$ C_{vm} $
\pagebreak

$ \beta $
\pagebreak

\[ \left( \theta_{ij}^{T} + \theta_{ij}^{B} + \theta_{ij}^{LS} \right) \lambda_{ij} \]
\pagebreak

\[ \lambda_{ij} = \mathrm{exp} \left( - \sqrt{\frac{r_{ij}^3 \rho_c}{16 \sigma}} \mathrm{ln} \left(\frac{h_0}{h_f}\right) \epsilon_c^{1/3}/r_{ij}^{2/3} \right)\;, \]
\pagebreak

\[ \theta_{ij}^{T} = C_1 \pi (d_i + d_j)^{2} \epsilon_c^{1/3} \sqrt{d_{i}^{2/3} + d_{j}^{2/3}}\;, \]
\pagebreak

\[ \theta_{ij}^{B} = S_{ij} \left| u_{ri} - u_{rj} \right|\;, \]
\pagebreak

\[ u_{ri} = \sqrt{2.14 \sigma / \left(\rho_c d_i \right) + 0.505 g d_i}\;, \]
\pagebreak

\[ r_{ij} = \left( \frac{1}{d_i} + \frac{1}{d_j} \right)^{-1} \]
\pagebreak

\[ S_{ij} = \frac{\pi}{4} \left(d_i + d_j\right)^{2}\;. \]
\pagebreak

$ \theta_{ij}^{T} $
\pagebreak

$ \theta_{ij}^{B} $
\pagebreak

$ \theta_{ij}^{LS} $
\pagebreak

$ \lambda_{ij} $
\pagebreak

$ r_{ij} $
\pagebreak

$ h_0 $
\pagebreak

$ h_f $
\pagebreak

$ u_{ri} $
\pagebreak

$ S_{ij} $
\pagebreak

\[ \frac{60}{v_j} \left(\frac{v_i}{v_j}\right)^{2} \left(1 - \frac{v_i}{v_j}\right)^{2} \]
\pagebreak

\[ wf = (1 - \alpha) - \alpha cos(2 \pi t/m); \]
\pagebreak

$ m $
\pagebreak

\[ U_p = \frac{n \phi}{\rho |Sf| \delta} \]
\pagebreak

$ \delta $
\pagebreak

$ \lambda $
\pagebreak

\[ \lambda = a(1 - \lambda)^b - c \lambda \dot{\gamma}^d \]
\pagebreak

\[ \mu = \frac{\mu_{\infty}}{{1 - K \lambda}^2} \]
\pagebreak

\[ K = 1 - \sqrt{\frac{\mu_{\infty}}{\mu_{0}}} \]
\pagebreak

$ b $
\pagebreak

$ \dot{\gamma} $
\pagebreak

$ \mu_{0} $
\pagebreak

$ \lambda = 1 $
\pagebreak

$ \mu_{\infty} $
\pagebreak

$ \lambda = 0 $
\pagebreak

\[ \phi_{Yi} = c A (Y_i - Y_{i,n}) \]
\pagebreak

$ \phi_{Yi} $
\pagebreak

$ Y_i $
\pagebreak

$ Y_{i,n} $
\pagebreak

\[ \nabla(e_p) = \nabla_\perp C_p(p, T) + \frac{e_p - e_c}{\Delta} \]
\pagebreak

$ e_p $
\pagebreak

$ e_c $
\pagebreak

$ T $
\pagebreak

$ C_p $
\pagebreak

$Su$
\pagebreak

\[ Su = \left( \sum \alpha_i \phi^i \right) \left( \frac{T}{T_{ref}} \right)^{\left( \sum \beta_j \phi^j \right)} \]
\pagebreak

$\phi$
\pagebreak

$\beta$
\pagebreak

\[ \kappa = 1000 - 0.05 T + 0.003 T^2 \]
\pagebreak

\[ \rho = 1000 - 0.05 T + 0.003 T^2 \]
\pagebreak

\[ 1/\rho = C_0 + C_1 T + C_2 T^2 - C_3 p - C_4 p T \]
\pagebreak

\[ Cp = 1000 - 0.05 T + 0.003 T^2 \]
\pagebreak

\[ ln(mu) = \sum_{i=1}^N \left( a[i] * ln(T)^{i-1} \right) \]
\pagebreak

\[ ln(kappa) = \sum_{i=1}^N \left( b[i] * ln(T)^{i-1} \right) \]
\pagebreak

\[ \mu = 1000 - 0.05 ln(T) + 0.003 ln(T)^2 \]
\pagebreak

\[ \kappa = 2000 - 0.15 ln(T) + 0.023 ln(T)^2 \]
\pagebreak

\[ \mu = 1000 - 0.05 T + 0.003 T^2 \]
\pagebreak

\[ \kappa = 2000 - 0.15 T + 0.023 T^2 \]
\pagebreak

\[ \mu = A_s \frac{\sqrt{T}}{1 + T_s / T} \]
\pagebreak

\[ \mu = \mu_0 \exp \left(\frac{-C_1 ( T - T_r )}{C_2 + T - T_r}\right) \]
\pagebreak

\begin{eqnarray*} 51104 + 2044 T & T > 295 & T < 373 \\ 255510 & T > 373 & \end{eqnarray*}
\pagebreak

\[ h_m = D_{ab} \frac{Sh}{L} \]
\pagebreak

$ D_{ab} $
\pagebreak

$ L $
\pagebreak

$ Sh $
\pagebreak

\begin{eqnarray*} 0.664 Re^\frac{1}{2} Sc^\frac{1}{3} & Re < 5.0E+05 \\ 0.037 Re^\frac{4}{5} Sc^\frac{1}{3} & Re > 5.0E+05 \end{eqnarray*}
\pagebreak

$ Re $
\pagebreak

$ Sc $
\pagebreak

\[ htc_p = \frac{0.664 Re^{0.5} Pr^{0.333} \kappa_p}{L} \]
\pagebreak

\[ htc_p = \frac{0.037 Re^{0.8} Pr^{0.333} \kappa_p}{L} \]
\pagebreak

$ htc_p $
\pagebreak

$ Pr $
\pagebreak

$ \kappa_p $
\pagebreak

$ Q $
\pagebreak

$ q $
\pagebreak

$ Ta $
\pagebreak

\[ \frac{p_{tot}}{p}=\left[ 1+ \frac{k-1}{2}\;M^2 \right]^{\frac{k}{k-1}} \]
\pagebreak

$k=c_p/c_v$
\pagebreak

$M=V/c$
\pagebreak

$c$
\pagebreak

\[ r = pBack/p_{tot} \]
\pagebreak

$k=1.4$
\pagebreak

$ r<0.5$
\pagebreak

$ r>=1 $
\pagebreak

$M_{outlet}$
\pagebreak

\[ c1\frac{A_{outlet}}{A_1}=\frac{1}{M_{outlet}}\left[\frac{1+\frac{k-1}{2} M_{outlet}^2}{1+\frac{k-1}{2}}\right]^{\frac{k+1}{2(k-1)}} \]
\pagebreak

$c1$
\pagebreak

$A_{outlet}$
\pagebreak

$A_1$
\pagebreak

\[ M_{outlet} = \frac{A_1} {c1\;A_{outlet}} \sqrt{\frac{2}{k-1}\left[r^\frac{2}{k}-r^\frac{k+1}{k} \right]} \]
\pagebreak

\[ \alpha_t = \frac{\mu_t}{Pr_t} \]
\pagebreak

$ \alpha_t$
\pagebreak

$ \mu_t $
\pagebreak

$ Pr_t $
\pagebreak

\[ weight = (1-sigma) w_1 + sigma w_2 \]
\pagebreak

$ sigma $
\pagebreak

$ w_1 $
\pagebreak

$ w_2 $
\pagebreak

\[ \Delta p = -(D \mu U + 0.5 I \rho |U|^2 )L \]
\pagebreak

$ \mu $
\pagebreak

$ D $
\pagebreak

$ epsilon $
\pagebreak

\[ u_\tau = (u_{\tau,v}^n + u_{\tau,l}^n)^{1/n} \]
\pagebreak

$ u_\tau $
\pagebreak

$ u_{\tau,v} $
\pagebreak

$ u_{\tau,l} $
\pagebreak

\[ y^+ = u^+ + \frac{1}{E} \left[exp(\kappa u^+) - 1 - \kappa u^+\, - 0.5 (\kappa u^+)^2 - \frac{1}{6} (\kappa u^+)^3\right] \]
\pagebreak

$ y^+ $
\pagebreak

$ u^+ $
\pagebreak

\[ \omega = sqrt(\omega_{vis}^2 + \omega_{log}^2) \]
\pagebreak

$ \omega_{vis} $
\pagebreak

$ \omega_{log} $
\pagebreak

\[ \epsilon_p = \frac{C_{\mu}^{0.75} k^{1.5}}{L} \]
\pagebreak

$ \epsilon_p $
\pagebreak

$\omega$
\pagebreak

\[ \omega_p = \frac{k^{0.5}}{C_{\mu}^{0.25} L} \]
\pagebreak

$ \omega_p $
\pagebreak

\[ \ddt{T} = \div \left( D_T \grad T \right) \]
\pagebreak

$ D_T $
\pagebreak

\[ \laplacian \Phi = \div(\vec{U}) \]
\pagebreak

$ \Phi $
\pagebreak

\[ \laplacian p + \div(\div(\vec{U}\otimes\vec{U})) = 0 \]
\pagebreak

\[ \laplacian p + \div(\vec{F}\cdot\div(\vec{U}\otimes\vec{U})) = 0 \]
\pagebreak

$\vec{F}$
\pagebreak

\[ \vec{F} = \hat{\vec{U}}\otimes\hat{\vec{U}} \]
\pagebreak

\[ \ddt{T} + \div \left(\vec{U} T\right) - \div \left(D_T \grad T \right) = S_{T} \]
\pagebreak

$ S_T $
\pagebreak

$ pexp $
\pagebreak

$ texp $
\pagebreak

$ Su = a_{0}(1+a_{1}x+K+..a_{i}x^{i}..+a_{6}x^{6}) (p/p_{ref})^{pexp} (T/T_{ref})^{texp} $
\pagebreak

$ a_{i} $
\pagebreak

\[ R = -\frac{1}{2} \rho \vert \dwea{\vec{U}} \vert \dwea{\vec{U}}.D \]
\pagebreak

$ m^{-1} $
\pagebreak

$ G_{R} $
\pagebreak

$ \kappa-\epsilon $
\pagebreak

$ G_{R} = C_{s}\beta_{\nu} \mu_{eff} A_{w}^{2}(\dwea{\vec{U}}-\dwea{\vec{U}_{s}})^2 + \frac{1}{2} \rho \vert \dwea{\vec{U}} \vert \dwea{\vec{U}}.T.\dwea{\vec{U}} $
\pagebreak

$ C_{s} $
\pagebreak

$ \beta_{\nu} $
\pagebreak

$ \mu_{eff} $
\pagebreak

$ A_{w}^{2}$
\pagebreak

$ \dwea{\vec{U}_{s}} $
\pagebreak

$ \frac{1}{2}. \dwea{\vec{U}} $
\pagebreak

$ C_{1} G_{R} $
\pagebreak

$ n = N - \hat{\dwea{\vec{U}}}.n_{s}.\hat{\dwea{\vec{U}}} $
\pagebreak

$ n_{r} = \sqrt{n} $
\pagebreak

$ \hat{\dwea{\vec{U}}} = \dwea{\vec{U}} / \vert \dwea{\vec{U}} \vert $
\pagebreak

$ b = \hat{\dwea{\vec{U}}}.B.\hat{\dwea{\vec{U}}} / n_{r} $
\pagebreak

$ B $
\pagebreak

$ N $
\pagebreak

$ n_{s} $
\pagebreak

$ \Xi_{sub} $
\pagebreak

\[ \Xi_{{sub}_{eq}} = 1 + max(2.2 \sqrt{b}, min(0.34 \frac{\vert \dwea{\vec{U}} \vert}{{\vec{U}}^{'}}, 1.6)) \times min(\frac{n}{4}, 1) \]
\pagebreak

$ G_{sub} $
\pagebreak

\[ G_{sub} = k_{1} /frac{\vert \dwea{\vec{U}} \vert}{L_{obs}} \frac{/Xi_{{sub}_{eq}}-1}{/Xi_{sub}} \]
\pagebreak

\[ - k_{1} /frac{\vert \dwea{\vec{U}} \vert}{L_{sub}} \frac{\Xi_{sub}-1}{\Xi_{sub}} \]
\pagebreak

$ G_{in} $
\pagebreak

$\Xi_{eq}$
\pagebreak

$\Xi_{eq} = 1 + (1 + 2\Xi_{coeff}(0.5 - \dwea{b}))(\Xi^* - 1)$
\pagebreak

$ \dwea{b} $
\pagebreak

$ \Xi_{coeff} $
\pagebreak

$ \Xi^* $
\pagebreak

\[ \Xi^* = \frac {R}{R - G_\eta - G_{in}} \]
\pagebreak

$ G_\eta $
\pagebreak

$ G_{in} = \kappa \rho_{u}/\rho_{b} $
\pagebreak

\[ R = G_\eta \frac{\Xi_{\eta_{eq}}}{\Xi_{\eta_{eq}} - 1} + G_{in} \frac{\Xi_{{in}_{eq}}}{\Xi_{{in}_{eq}} - 1} \]
\pagebreak

$ \Xi_{\eta_{eq}} $
\pagebreak

$ \Xi_{{in}_{eq}} $
\pagebreak

\[ \rho = \psi p \]
\pagebreak

\[ \ddt{Cs} + \div \left(\vec{U} Cs\right) - \div \left(D_T \grad Cs \right) = 0 \]
\pagebreak

$ Cs $
\pagebreak

$ Ds $
\pagebreak

\[ rho_{k} = 1 - beta(T - T_{ref}) \]
\pagebreak

$ rho_{k} $
\pagebreak

\[ \frac{beta(T - T_{ref})}{rho_{ref}} << 1 \]
\pagebreak

\[ \div \vec{U} = 0 \]
\pagebreak

\[ \ddt{\vec{U}} + \div \left( \vec{U} \vec{U} \right) - \div \left(\nu \grad \vec{U} \right) = - \grad p \]
\pagebreak

\[ \ddt{\vec{U}} + \div \left( \vec{U} \vec{U} \right) - \div \gvec{R} = - \grad p + \vec{S}_U \]
\pagebreak

$ \vec{R} $
\pagebreak

$ \vec{S}_U $
\pagebreak

\[ \ddt{\vec{U}} + \div \left( \vec{U} \vec{U} \right) - \div \gvec{R} = - \grad p \]
\pagebreak

\[ \div \left( \vec{U} \vec{U} \right) - \div \gvec{R} = - \grad p + \vec{S}_U \]
\pagebreak

\[ Flux = C \sqrt{\frac{M}{2 \pi R T_{activate}}}(p - p_{sat}) \]
\pagebreak

$ Flux $
\pagebreak

$ M $
\pagebreak

$ T_{activate} $
\pagebreak

$ C $
\pagebreak

\[ \frac{dp}{dT} = - \frac{L}{T (\nu_v - \nu_l)} \]
\pagebreak

$ \nu_v $
\pagebreak

$ \nu_l $
\pagebreak

\[ Flux = 2 \frac{C}{2 - C} \sqrt{\frac{M}{2 \pi R T_{activate}}} L (\rho_{v}*\rho_{l}/(\rho_{l} - \rho_{v})) (T - T_{activate})/T_{activate} \]
\pagebreak

\[ \dot{m} = C \rho \alpha (T - T_{activate})/T_{activate} \]
\pagebreak

\[ T > T_{activate} \]
\pagebreak

\[ mDot = 0.0 \]
\pagebreak

\[ T < T_{activate} \]
\pagebreak

\[ \dot{m} = -C \rho \alpha (T_{activate} - T)/T_{activate} \]
\pagebreak

\[ \dot{m} = 0.0 \]
\pagebreak

\end{document}
